Merge and update on jasmin extraction

proof/correctness/extraction/jindcpa.ec
@@ -1,10 +1,11 @@
 require import AllCore IntDiv CoreMap List.
 from Jasmin require import JModel.
 
-require import Array4 Array5 Array24 Array25 Array32 Array33 Array34 Array128
-               Array168 Array256 Array768.
-require import WArray20 WArray32 WArray33 WArray34 WArray40 WArray128
-               WArray168 WArray192 WArray200 WArray256 WArray512 WArray1536.
+require import Array4 Array5 Array24 Array25 Array32 Array33 Array34 Array64
+               Array128 Array168 Array256 Array768.
+require import WArray20 WArray32 WArray33 WArray34 WArray40 WArray64
+               WArray128 WArray168 WArray192 WArray200 WArray256 WArray512
+               WArray1536.
 
 abbrev roundconstants = Array24.of_list witness [W64.of_int 1;
 W64.of_int 32898; W64.of_int (-9223372036854742902);
@@ -90,7 +91,7 @@ W16.of_int 1522; W16.of_int 1628].
 
 
 module M = {
-  proc _poly_csubq (rp:W16.t Array256.t) : W16.t Array256.t = {
+  proc poly_csubq (rp:W16.t Array256.t) : W16.t Array256.t = {
     
     var i:W64.t;
     var t:W16.t;
@@ -111,7 +112,7 @@ module M = {
     return (rp);
   }
   
-  proc _poly_compress (rp:W64.t, a:W16.t Array256.t) : W16.t Array256.t = {
+  proc poly_compress (rp:W64.t, a:W16.t Array256.t) : W16.t Array256.t = {
     
     var i:W64.t;
     var j:W64.t;
@@ -119,7 +120,7 @@ module M = {
     var d0:W32.t;
     var d1:W32.t;
     
-    a <@ _poly_csubq (a);
+    a <@ poly_csubq (a);
     i <- (W64.of_int 0);
     j <- (W64.of_int 0);
     
@@ -148,7 +149,7 @@ module M = {
     return (a);
   }
   
-  proc _poly_decompress (rp:W16.t Array256.t, ap:W64.t) : W16.t Array256.t = {
+  proc poly_decompress (rp:W16.t Array256.t, ap:W64.t) : W16.t Array256.t = {
     
     var i:W64.t;
     var j:W64.t;
@@ -180,7 +181,42 @@ module M = {
     return (rp);
   }
   
-  proc _poly_frombytes (rp:W16.t Array256.t, ap:W64.t) : W16.t Array256.t = {
+  proc poly_tobytes (rp:W64.t, a:W16.t Array256.t) : W16.t Array256.t = {
+    
+    var i:W64.t;
+    var j:W64.t;
+    var t0:W16.t;
+    var t1:W16.t;
+    var d:W16.t;
+    
+    a <@ poly_csubq (a);
+    i <- (W64.of_int 0);
+    j <- (W64.of_int 0);
+    
+    while ((i \ult (W64.of_int 256))) {
+      t0 <- a.[(W64.to_uint i)];
+      i <- (i + (W64.of_int 1));
+      t1 <- a.[(W64.to_uint i)];
+      i <- (i + (W64.of_int 1));
+      d <- t0;
+      d <- (d `&` (W16.of_int 255));
+      Glob.mem <- storeW8 Glob.mem (W64.to_uint (rp + j)) (truncateu8 d);
+      j <- (j + (W64.of_int 1));
+      t0 <- (t0 `>>` (W8.of_int 8));
+      d <- t1;
+      d <- (d `&` (W16.of_int 15));
+      d <- (d `<<` (W8.of_int 4));
+      d <- (d `|` t0);
+      Glob.mem <- storeW8 Glob.mem (W64.to_uint (rp + j)) (truncateu8 d);
+      j <- (j + (W64.of_int 1));
+      t1 <- (t1 `>>` (W8.of_int 4));
+      Glob.mem <- storeW8 Glob.mem (W64.to_uint (rp + j)) (truncateu8 t1);
+      j <- (j + (W64.of_int 1));
+    }
+    return (a);
+  }
+  
+  proc poly_frombytes (rp:W16.t Array256.t, ap:W64.t) : W16.t Array256.t = {
     var aux: int;
     
     var i:int;
@@ -216,7 +252,7 @@ module M = {
     return (rp);
   }
   
-  proc _poly_tomsg (rp:W64.t, a:W16.t Array256.t) : W16.t Array256.t = {
+  proc poly_tomsg (rp:W64.t, a:W16.t Array256.t) : W16.t Array256.t = {
     var aux: int;
     
     var r:W8.t;
@@ -225,7 +261,7 @@ module M = {
     var t:W16.t;
     var d:W32.t;
     
-    a <@ _poly_csubq (a);
+    a <@ poly_csubq (a);
     i <- 0;
     while (i < 32) {
       r <- (W8.of_int 0);
@@ -248,7 +284,7 @@ module M = {
     return (a);
   }
   
-  proc _poly_frommsg (rp:W16.t Array256.t, ap:W64.t) : W16.t Array256.t = {
+  proc poly_frommsg (rp:W16.t Array256.t, ap:W64.t) : W16.t Array256.t = {
     var aux: int;
     
     var i:int;
@@ -303,7 +339,7 @@ module M = {
     return (rp);
   }
   
-  proc _poly_add2 (rp:W16.t Array256.t, bp:W16.t Array256.t) : W16.t Array256.t = {
+  proc poly_add2 (rp:W16.t Array256.t, bp:W16.t Array256.t) : W16.t Array256.t = {
     
     var i:W64.t;
     var a:W16.t;
@@ -322,8 +358,8 @@ module M = {
     return (rp);
   }
   
-  proc _poly_sub (rp:W16.t Array256.t, ap:W16.t Array256.t,
-                  bp:W16.t Array256.t) : W16.t Array256.t = {
+  proc poly_sub (rp:W16.t Array256.t, ap:W16.t Array256.t,
+                 bp:W16.t Array256.t) : W16.t Array256.t = {
     
     var i:W64.t;
     var a:W16.t;
@@ -342,7 +378,7 @@ module M = {
     return (rp);
   }
   
-  proc __fqmul (a:W16.t, b:W16.t) : W16.t = {
+  proc fqmul (a:W16.t, b:W16.t) : W16.t = {
     
     var r:W16.t;
     var ad:W32.t;
@@ -364,7 +400,7 @@ module M = {
     return (r);
   }
   
-  proc __barrett_reduce (a:W16.t) : W16.t = {
+  proc barrett_reduce (a:W16.t) : W16.t = {
     
     var r:W16.t;
     var t:W32.t;
@@ -379,7 +415,7 @@ module M = {
     return (r);
   }
   
-  proc __poly_reduce (rp:W16.t Array256.t) : W16.t Array256.t = {
+  proc poly_reduce (rp:W16.t Array256.t) : W16.t Array256.t = {
     
     var j:W64.t;
     var t:W16.t;
@@ -388,14 +424,14 @@ module M = {
     
     while ((j \ult (W64.of_int 256))) {
       t <- rp.[(W64.to_uint j)];
-      t <@ __barrett_reduce (t);
+      t <@ barrett_reduce (t);
       rp.[(W64.to_uint j)] <- t;
       j <- (j + (W64.of_int 1));
     }
     return (rp);
   }
   
-  proc _poly_ntt (rp:W16.t Array256.t) : W16.t Array256.t = {
+  proc poly_ntt (rp:W16.t Array256.t) : W16.t Array256.t = {
     
     var zetasp:W16.t Array128.t;
     var zetasctr:W64.t;
@@ -425,7 +461,7 @@ module M = {
         while ((j \ult cmp)) {
           offset <- (j + len);
           t <- rp.[(W64.to_uint offset)];
-          t <@ __fqmul (t, zeta_0);
+          t <@ fqmul (t, zeta_0);
           s <- rp.[(W64.to_uint j)];
           m <- s;
           m <- (m - t);
@@ -438,11 +474,11 @@ module M = {
       }
       len <- (len `>>` (W8.of_int 1));
     }
-    rp <@ __poly_reduce (rp);
+    rp <@ poly_reduce (rp);
     return (rp);
   }
   
-  proc _poly_invntt (rp:W16.t Array256.t) : W16.t Array256.t = {
+  proc poly_invntt (rp:W16.t Array256.t) : W16.t Array256.t = {
     
     var zetasp:W16.t Array128.t;
     var zetasctr:W64.t;
@@ -474,10 +510,10 @@ module M = {
           s <- rp.[(W64.to_uint offset)];
           t <- rp.[(W64.to_uint j)];
           m <- (s + t);
-          m <@ __barrett_reduce (m);
+          m <@ barrett_reduce (m);
           rp.[(W64.to_uint j)] <- m;
           t <- (t - s);
-          t <@ __fqmul (t, zeta_0);
+          t <@ fqmul (t, zeta_0);
           rp.[(W64.to_uint offset)] <- t;
           j <- (j + (W64.of_int 1));
         }
@@ -490,15 +526,15 @@ module M = {
     
     while ((j \ult (W64.of_int 256))) {
       t <- rp.[(W64.to_uint j)];
-      t <@ __fqmul (t, zeta_0);
+      t <@ fqmul (t, zeta_0);
       rp.[(W64.to_uint j)] <- t;
       j <- (j + (W64.of_int 1));
     }
     return (rp);
   }
   
-  proc _poly_basemul (rp:W16.t Array256.t, ap:W16.t Array256.t,
-                      bp:W16.t Array256.t) : W16.t Array256.t = {
+  proc poly_basemul (rp:W16.t Array256.t, ap:W16.t Array256.t,
+                     bp:W16.t Array256.t) : W16.t Array256.t = {
     
     var srp:W16.t Array256.t;
     var zetasctr:W64.t;
@@ -528,12 +564,12 @@ module M = {
       a1 <- ap.[(W64.to_uint i)];
       b1 <- bp.[(W64.to_uint i)];
       i <- (i - (W64.of_int 1));
-      r0 <@ __fqmul (a1, b1);
-      r0 <@ __fqmul (r0, zeta_0);
-      t <@ __fqmul (a0, b0);
+      r0 <@ fqmul (a1, b1);
+      r0 <@ fqmul (r0, zeta_0);
+      t <@ fqmul (a0, b0);
       r0 <- (r0 + t);
-      r1 <@ __fqmul (a0, b1);
-      t <@ __fqmul (a1, b0);
+      r1 <@ fqmul (a0, b1);
+      t <@ fqmul (a1, b0);
       r1 <- (r1 + t);
       rp <- srp;
       rp.[(W64.to_uint i)] <- r0;
@@ -548,12 +584,12 @@ module M = {
       a1 <- ap.[(W64.to_uint i)];
       b1 <- bp.[(W64.to_uint i)];
       i <- (i - (W64.of_int 1));
-      r0 <@ __fqmul (a1, b1);
-      r0 <@ __fqmul (r0, zeta_0);
-      t <@ __fqmul (a0, b0);
+      r0 <@ fqmul (a1, b1);
+      r0 <@ fqmul (r0, zeta_0);
+      t <@ fqmul (a0, b0);
       r0 <- (r0 + t);
-      r1 <@ __fqmul (a0, b1);
-      t <@ __fqmul (a1, b0);
+      r1 <@ fqmul (a0, b1);
+      t <@ fqmul (a1, b0);
       r1 <- (r1 + t);
       rp <- srp;
       rp.[(W64.to_uint i)] <- r0;
@@ -565,7 +601,25 @@ module M = {
     return (rp);
   }
   
-  proc __index (x:int, y:int) : int = {
+  proc poly_frommont (rp:W16.t Array256.t) : W16.t Array256.t = {
+    
+    var dmont:W16.t;
+    var i:W64.t;
+    var r:W16.t;
+    
+    dmont <- (W16.of_int 1353);
+    i <- (W64.of_int 0);
+    
+    while ((i \ult (W64.of_int 256))) {
+      r <- rp.[(W64.to_uint i)];
+      r <@ fqmul (r, dmont);
+      rp.[(W64.to_uint i)] <- r;
+      i <- (i + (W64.of_int 1));
+    }
+    return (rp);
+  }
+  
+  proc index (x:int, y:int) : int = {
     
     var r:int;
     
@@ -573,7 +627,7 @@ module M = {
     return (r);
   }
   
-  proc __theta (a:W64.t Array25.t) : W64.t Array25.t = {
+  proc theta (a:W64.t Array25.t) : W64.t Array25.t = {
     var aux_1: bool;
     var aux_0: bool;
     var aux: int;
@@ -619,7 +673,7 @@ module M = {
     return (a);
   }
   
-  proc __keccakRhoOffsets (i:int) : int = {
+  proc keccakRhoOffsets (i:int) : int = {
     var aux: int;
     
     var r:int;
@@ -646,7 +700,7 @@ module M = {
     return (r);
   }
   
-  proc __rho (a:W64.t Array25.t) : W64.t Array25.t = {
+  proc rho (a:W64.t Array25.t) : W64.t Array25.t = {
     var aux_1: bool;
     var aux_0: bool;
     var aux: int;
@@ -663,8 +717,8 @@ module M = {
     while (x < 5) {
       y <- 0;
       while (y < 5) {
-        i <@ __index (x, y);
-        z <@ __keccakRhoOffsets (i);
+        i <@ index (x, y);
+        z <@ keccakRhoOffsets (i);
         (aux_1, aux_0, aux_2) <- ROL_64 a.[i] (W8.of_int z);
          _0 <- aux_1;
          _1 <- aux_0;
@@ -676,7 +730,7 @@ module M = {
     return (a);
   }
   
-  proc __pi (a:W64.t Array25.t) : W64.t Array25.t = {
+  proc pi (a:W64.t Array25.t) : W64.t Array25.t = {
     var aux: int;
     
     var i:int;
@@ -696,7 +750,7 @@ module M = {
       y <- 0;
       while (y < 5) {
         t <- b.[(x + (5 * y))];
-        i <@ __index (y, ((2 * x) + (3 * y)));
+        i <@ index (y, ((2 * x) + (3 * y)));
         a.[i] <- t;
         y <- y + 1;
       }
@@ -705,7 +759,7 @@ module M = {
     return (a);
   }
   
-  proc __chi (a:W64.t Array25.t) : W64.t Array25.t = {
+  proc chi (a:W64.t Array25.t) : W64.t Array25.t = {
     var aux: int;
     
     var x:int;
@@ -717,12 +771,12 @@ module M = {
     while (y < 5) {
       x <- 0;
       while (x < 5) {
-        i <@ __index ((x + 1), y);
+        i <@ index ((x + 1), y);
         c.[x] <- a.[i];
         c.[x] <- (invw c.[x]);
-        i <@ __index ((x + 2), y);
+        i <@ index ((x + 2), y);
         c.[x] <- (c.[x] `&` a.[i]);
-        i <@ __index (x, y);
+        i <@ index (x, y);
         c.[x] <- (c.[x] `^` a.[i]);
         x <- x + 1;
       }
@@ -736,7 +790,7 @@ module M = {
     return (a);
   }
   
-  proc __iota (a:W64.t Array25.t, c:W64.t) : W64.t Array25.t = {
+  proc iota_0 (a:W64.t Array25.t, c:W64.t) : W64.t Array25.t = {
     
     
     
@@ -744,7 +798,7 @@ module M = {
     return (a);
   }
   
-  proc _keccakf1600_ref (state:W64.t Array25.t) : W64.t Array25.t = {
+  proc __keccakf1600_ref (state:W64.t Array25.t) : W64.t Array25.t = {
     
     var constptr:W64.t Array24.t;
     var rctr:W64.t;
@@ -752,19 +806,21 @@ module M = {
     constptr <- roundconstants;
     rctr <- (W64.of_int 0);
     
-    while ((rctr \ult (W64.of_int 24))) {
-      state <@ __theta (state);
-      state <@ __rho (state);
-      state <@ __pi (state);
-      state <@ __chi (state);
+    while ((rctr \ult (W64.of_int 192))) {
+      state <@ theta (state);
+      state <@ rho (state);
+      state <@ pi (state);
+      state <@ chi (state);
       constptr <- roundconstants;
-      state <@ __iota (state, constptr.[(W64.to_uint rctr)]);
-      rctr <- (rctr + (W64.of_int 1));
+      state <@ iota_0 (state,
+      (get64_direct (WArray192.init64 (fun i => constptr.[i]))
+      (W64.to_uint rctr)));
+      rctr <- (rctr + (W64.of_int 8));
     }
     return (state);
   }
   
-  proc __st0 (state:W64.t Array25.t) : W64.t Array25.t = {
+  proc st0 (state:W64.t Array25.t) : W64.t Array25.t = {
     var aux: int;
     
     var i:int;
@@ -777,8 +833,7 @@ module M = {
     return (state);
   }
   
-  proc _shake256_128_33 (out:W8.t Array128.t, in_0:W8.t Array33.t) : 
-  W8.t Array128.t = {
+  proc shake256_128_33 (out:W8.t Array128.t, in_0:W8.t Array33.t) : W8.t Array128.t = {
     var aux: int;
     
     var sout:W8.t Array128.t;
@@ -788,7 +843,7 @@ module M = {
     sout <- witness;
     state <- witness;
     sout <- out;
-    state <@ __st0 (state);
+    state <@ st0 (state);
     i <- 0;
     while (i < 33) {
       c <- in_0.[i];
@@ -806,7 +861,7 @@ module M = {
     Array25.init
     (WArray200.get64 (WArray200.set8 (WArray200.init64 (fun i => state.[i])) (136 - 1) (
     (get8 (WArray200.init64 (fun i => state.[i])) (136 - 1)) `^` (W8.of_int 128))));
-    state <@ _keccakf1600_ref (state);
+    state <@ __keccakf1600_ref (state);
     out <- sout;
     i <- 0;
     while (i < 128) {
@@ -817,14 +872,49 @@ module M = {
     return (out);
   }
   
-  proc _shake128_absorb34 (state:W64.t Array25.t, in_0:W8.t Array34.t) : 
+  proc sha3512_32 (out:W8.t Array64.t, in_0:W8.t Array32.t) : W8.t Array64.t = {
+    var aux: int;
+    
+    var state:W64.t Array25.t;
+    var i:int;
+    var c:W8.t;
+    state <- witness;
+    state <@ st0 (state);
+    i <- 0;
+    while (i < 32) {
+      c <- in_0.[i];
+      state <-
+      Array25.init
+      (WArray200.get64 (WArray200.set8 (WArray200.init64 (fun i => state.[i])) i (
+      (get8 (WArray200.init64 (fun i => state.[i])) i) `^` c)));
+      i <- i + 1;
+    }
+    state <-
+    Array25.init
+    (WArray200.get64 (WArray200.set8 (WArray200.init64 (fun i => state.[i])) 32 (
+    (get8 (WArray200.init64 (fun i => state.[i])) 32) `^` (W8.of_int 6))));
+    state <-
+    Array25.init
+    (WArray200.get64 (WArray200.set8 (WArray200.init64 (fun i => state.[i])) (72 - 1) (
+    (get8 (WArray200.init64 (fun i => state.[i])) (72 - 1)) `^` (W8.of_int 128))));
+    state <@ __keccakf1600_ref (state);
+    i <- 0;
+    while (i < 64) {
+      c <- (get8 (WArray200.init64 (fun i => state.[i])) i);
+      out.[i] <- c;
+      i <- i + 1;
+    }
+    return (out);
+  }
+  
+  proc shake128_absorb34 (state:W64.t Array25.t, in_0:W8.t Array34.t) : 
   W64.t Array25.t = {
     var aux: int;
     
     var i:int;
     var c:W8.t;
     
-    state <@ __st0 (state);
+    state <@ st0 (state);
     i <- 0;
     while (i < 34) {
       c <- in_0.[i];
@@ -845,14 +935,14 @@ module M = {
     return (state);
   }
   
-  proc _shake128_squeezeblock (state:W64.t Array25.t, out:W8.t Array168.t) : 
+  proc shake128_squeezeblock (state:W64.t Array25.t, out:W8.t Array168.t) : 
   W64.t Array25.t * W8.t Array168.t = {
     var aux: int;
     
     var i:int;
     var c:W8.t;
     
-    state <@ _keccakf1600_ref (state);
+    state <@ __keccakf1600_ref (state);
     i <- 0;
     while (i < 168) {
       c <- (get8 (WArray200.init64 (fun i => state.[i])) i);
@@ -862,7 +952,7 @@ module M = {
     return (state, out);
   }
   
-  proc _poly_getnoise (rp:W16.t Array256.t, seed:W8.t Array32.t, nonce:W8.t) : 
+  proc poly_getnoise (rp:W16.t Array256.t, seed:W8.t Array32.t, nonce:W8.t) : 
   W16.t Array256.t = {
     var aux: int;
     
@@ -887,7 +977,7 @@ module M = {
       k <- k + 1;
     }
     extseed.[32] <- nonce;
-    buf <@ _shake256_128_33 (buf, extseed);
+    buf <@ shake256_128_33 (buf, extseed);
     rp <- srp;
     i <- (W64.of_int 0);
     j <- (W64.of_int 0);
@@ -922,9 +1012,9 @@ module M = {
     return (rp);
   }
   
-  proc __polyvec_topolys (pv:W16.t Array768.t) : W16.t Array256.t *
-                                                 W16.t Array256.t *
-                                                 W16.t Array256.t = {
+  proc polyvec_topolys (pv:W16.t Array768.t) : W16.t Array256.t *
+                                               W16.t Array256.t *
+                                               W16.t Array256.t = {
     
     var r0:W16.t Array256.t;
     var r1:W16.t Array256.t;
@@ -963,8 +1053,8 @@ module M = {
     return (r0, r1, r2);
   }
   
-  proc __polyvec_frompolys (p0:W16.t Array256.t, p1:W16.t Array256.t,
-                            p2:W16.t Array256.t) : W16.t Array768.t = {
+  proc polyvec_frompolys (p0:W16.t Array256.t, p1:W16.t Array256.t,
+                          p2:W16.t Array256.t) : W16.t Array768.t = {
     
     var r:W16.t Array768.t;
     var i:W64.t;
@@ -999,7 +1089,26 @@ module M = {
     return (r);
   }
   
-  proc __polyvec_frombytes (ap:W64.t) : W16.t Array768.t = {
+  proc polyvec_tobytes (rp:W64.t, a:W16.t Array768.t) : unit = {
+    
+    var a0:W16.t Array256.t;
+    var a1:W16.t Array256.t;
+    var a2:W16.t Array256.t;
+    var pp:W64.t;
+    a0 <- witness;
+    a1 <- witness;
+    a2 <- witness;
+    (a0, a1, a2) <@ polyvec_topolys (a);
+    pp <- rp;
+    a0 <@ poly_tobytes (pp, a0);
+    pp <- (pp + (W64.of_int 384));
+    a1 <@ poly_tobytes (pp, a1);
+    pp <- (pp + (W64.of_int 384));
+    a2 <@ poly_tobytes (pp, a2);
+    return ();
+  }
+  
+  proc polyvec_frombytes (ap:W64.t) : W16.t Array768.t = {
     
     var r:W16.t Array768.t;
     var pp:W64.t;
@@ -1011,16 +1120,16 @@ module M = {
     r1 <- witness;
     r2 <- witness;
     pp <- ap;
-    r0 <@ _poly_frombytes (r0, pp);
+    r0 <@ poly_frombytes (r0, pp);
     pp <- (pp + (W64.of_int 384));
-    r1 <@ _poly_frombytes (r1, pp);
+    r1 <@ poly_frombytes (r1, pp);
     pp <- (pp + (W64.of_int 384));
-    r2 <@ _poly_frombytes (r2, pp);
-    r <@ __polyvec_frompolys (r0, r1, r2);
+    r2 <@ poly_frombytes (r2, pp);
+    r <@ polyvec_frompolys (r0, r1, r2);
     return (r);
   }
   
-  proc __polyvec_csubq (r:W16.t Array768.t) : W16.t Array768.t = {
+  proc polyvec_csubq (r:W16.t Array768.t) : W16.t Array768.t = {
     
     var r0:W16.t Array256.t;
     var r1:W16.t Array256.t;
@@ -1028,15 +1137,15 @@ module M = {
     r0 <- witness;
     r1 <- witness;
     r2 <- witness;
-    (r0, r1, r2) <@ __polyvec_topolys (r);
-    r0 <@ _poly_csubq (r0);
-    r1 <@ _poly_csubq (r1);
-    r2 <@ _poly_csubq (r2);
-    r <@ __polyvec_frompolys (r0, r1, r2);
+    (r0, r1, r2) <@ polyvec_topolys (r);
+    r0 <@ poly_csubq (r0);
+    r1 <@ poly_csubq (r1);
+    r2 <@ poly_csubq (r2);
+    r <@ polyvec_frompolys (r0, r1, r2);
     return (r);
   }
   
-  proc __polyvec_compress (rp:W64.t, a:W16.t Array768.t) : unit = {
+  proc polyvec_compress (rp:W64.t, a:W16.t Array768.t) : unit = {
     var aux: int;
     
     var i:W64.t;
@@ -1050,7 +1159,7 @@ module M = {
     t <- witness;
     i <- (W64.of_int 0);
     j <- (W64.of_int 0);
-    aa <@ __polyvec_csubq (a);
+    aa <@ polyvec_csubq (a);
     
     while ((i \ult (W64.of_int 768))) {
       k <- 0;
@@ -1096,7 +1205,7 @@ module M = {
     return ();
   }
   
-  proc __polyvec_decompress (ap:W64.t) : W16.t Array768.t = {
+  proc polyvec_decompress (ap:W64.t) : W16.t Array768.t = {
     var aux: int;
     
     var r:W16.t Array768.t;
@@ -1148,7 +1257,7 @@ module M = {
     return (r);
   }
   
-  proc __polyvec_add2 (r:W16.t Array768.t, b:W16.t Array768.t) : W16.t Array768.t = {
+  proc polyvec_add2 (r:W16.t Array768.t, b:W16.t Array768.t) : W16.t Array768.t = {
     
     var r0:W16.t Array256.t;
     var r1:W16.t Array256.t;
@@ -1162,16 +1271,16 @@ module M = {
     r0 <- witness;
     r1 <- witness;
     r2 <- witness;
-    (r0, r1, r2) <@ __polyvec_topolys (r);
-    (b0, b1, b2) <@ __polyvec_topolys (b);
-    r0 <@ _poly_add2 (r0, b0);
-    r1 <@ _poly_add2 (r1, b1);
-    r2 <@ _poly_add2 (r2, b2);
-    r <@ __polyvec_frompolys (r0, r1, r2);
+    (r0, r1, r2) <@ polyvec_topolys (r);
+    (b0, b1, b2) <@ polyvec_topolys (b);
+    r0 <@ poly_add2 (r0, b0);
+    r1 <@ poly_add2 (r1, b1);
+    r2 <@ poly_add2 (r2, b2);
+    r <@ polyvec_frompolys (r0, r1, r2);
     return (r);
   }
   
-  proc __polyvec_pointwise_acc (a:W16.t Array768.t, b:W16.t Array768.t) : 
+  proc polyvec_pointwise_acc (a:W16.t Array768.t, b:W16.t Array768.t) : 
   W16.t Array256.t = {
     
     var r:W16.t Array256.t;
@@ -1190,18 +1299,18 @@ module M = {
     b2 <- witness;
     r <- witness;
     t <- witness;
-    (a0, a1, a2) <@ __polyvec_topolys (a);
-    (b0, b1, b2) <@ __polyvec_topolys (b);
-    r <@ _poly_basemul (r, a0, b0);
-    t <@ _poly_basemul (t, a1, b1);
-    r <@ _poly_add2 (r, t);
-    t <@ _poly_basemul (t, a2, b2);
-    r <@ _poly_add2 (r, t);
-    r <@ __poly_reduce (r);
+    (a0, a1, a2) <@ polyvec_topolys (a);
+    (b0, b1, b2) <@ polyvec_topolys (b);
+    r <@ poly_basemul (r, a0, b0);
+    t <@ poly_basemul (t, a1, b1);
+    r <@ poly_add2 (r, t);
+    t <@ poly_basemul (t, a2, b2);
+    r <@ poly_add2 (r, t);
+    r <@ poly_reduce (r);
     return (r);
   }
   
-  proc __polyvec_ntt (r:W16.t Array768.t) : W16.t Array768.t = {
+  proc polyvec_ntt (r:W16.t Array768.t) : W16.t Array768.t = {
     
     var r0:W16.t Array256.t;
     var r1:W16.t Array256.t;
@@ -1209,15 +1318,15 @@ module M = {
     r0 <- witness;
     r1 <- witness;
     r2 <- witness;
-    (r0, r1, r2) <@ __polyvec_topolys (r);
-    r0 <@ _poly_ntt (r0);
-    r1 <@ _poly_ntt (r1);
-    r2 <@ _poly_ntt (r2);
-    r <@ __polyvec_frompolys (r0, r1, r2);
+    (r0, r1, r2) <@ polyvec_topolys (r);
+    r0 <@ poly_ntt (r0);
+    r1 <@ poly_ntt (r1);
+    r2 <@ poly_ntt (r2);
+    r <@ polyvec_frompolys (r0, r1, r2);
     return (r);
   }
   
-  proc __polyvec_invntt (r:W16.t Array768.t) : W16.t Array768.t = {
+  proc polyvec_invntt (r:W16.t Array768.t) : W16.t Array768.t = {
     
     var r0:W16.t Array256.t;
     var r1:W16.t Array256.t;
@@ -1225,15 +1334,15 @@ module M = {
     r0 <- witness;
     r1 <- witness;
     r2 <- witness;
-    (r0, r1, r2) <@ __polyvec_topolys (r);
-    r0 <@ _poly_invntt (r0);
-    r1 <@ _poly_invntt (r1);
-    r2 <@ _poly_invntt (r2);
-    r <@ __polyvec_frompolys (r0, r1, r2);
+    (r0, r1, r2) <@ polyvec_topolys (r);
+    r0 <@ poly_invntt (r0);
+    r1 <@ poly_invntt (r1);
+    r2 <@ poly_invntt (r2);
+    r <@ polyvec_frompolys (r0, r1, r2);
     return (r);
   }
   
-  proc __polyvec_reduce (r:W16.t Array768.t) : W16.t Array768.t = {
+  proc polyvec_reduce (r:W16.t Array768.t) : W16.t Array768.t = {
     
     var r0:W16.t Array256.t;
     var r1:W16.t Array256.t;
@@ -1241,23 +1350,22 @@ module M = {
     r0 <- witness;
     r1 <- witness;
     r2 <- witness;
-    (r0, r1, r2) <@ __polyvec_topolys (r);
-    r0 <@ __poly_reduce (r0);
-    r1 <@ __poly_reduce (r1);
-    r2 <@ __poly_reduce (r2);
-    r <@ __polyvec_frompolys (r0, r1, r2);
+    (r0, r1, r2) <@ polyvec_topolys (r);
+    r0 <@ poly_reduce (r0);
+    r1 <@ poly_reduce (r1);
+    r2 <@ poly_reduce (r2);
+    r <@ polyvec_frompolys (r0, r1, r2);
     return (r);
   }
   
-  proc __rej_uniform (rp:W16.t Array256.t, offset:W64.t, buf:W8.t Array168.t) : 
+  proc rej_uniform (rp:W16.t Array256.t, offset:W64.t, buf:W8.t Array168.t) : 
   W64.t * W16.t Array256.t = {
     
     var ctr:W64.t;
     var pos:W64.t;
     var exit:W64.t;
-    var val1:W16.t;
+    var val:W16.t;
     var t:W16.t;
-    var val2:W16.t;
     var cnd0:W64.t;
     var cnd1:W64.t;
     
@@ -1266,32 +1374,19 @@ module M = {
     exit <- (W64.of_int 0);
     
     while ((exit = (W64.of_int 0))) {
-      val1 <- (zeroextu16 buf.[(W64.to_uint pos)]);
+      val <- (zeroextu16 buf.[(W64.to_uint pos)]);
       pos <- (pos + (W64.of_int 1));
       t <- (zeroextu16 buf.[(W64.to_uint pos)]);
-      val2 <- t;
-      val2 <- (val2 `>>` (W8.of_int 4));
-      t <- (t `&` (W16.of_int 15));
       t <- (t `<<` (W8.of_int 8));
-      val1 <- (val1 `|` t);
+      val <- (val `|` t);
       pos <- (pos + (W64.of_int 1));
-      t <- (zeroextu16 buf.[(W64.to_uint pos)]);
-      t <- (t `<<` (W8.of_int 4));
-      val2 <- (val2 `|` t);
-      pos <- (pos + (W64.of_int 1));
-      if ((val1 \ult (W16.of_int 3329))) {
-        rp.[(W64.to_uint ctr)] <- val1;
+      if ((val \ult (W16.of_int 63251))) {
+        t <- val;
+        t <- (t `>>` (W8.of_int 12));
+        t <- (t * (W16.of_int 3329));
+        val <- (val - t);
+        rp.[(W64.to_uint ctr)] <- val;
         ctr <- (ctr + (W64.of_int 1));
-      } else {
-        
-      }
-      if ((val2 \ult (W16.of_int 3329))) {
-        if ((ctr \ult (W64.of_int 256))) {
-          rp.[(W64.to_uint ctr)] <- val2;
-          ctr <- (ctr + (W64.of_int 1));
-        } else {
-          
-        }
       } else {
         
       }
@@ -1300,16 +1395,16 @@ module M = {
       cnd0 <- (cnd0 - (W64.of_int 1));
       cnd1 <- (W64.of_int 168);
       cnd1 <- (cnd1 - pos);
-      cnd1 <- (cnd1 - (W64.of_int 3));
+      cnd1 <- (cnd1 - (W64.of_int 2));
       exit <- (cnd0 `|` cnd1);
       exit <- (exit `>>` (W8.of_int 63));
     }
     return (ctr, rp);
   }
   
-  proc __gen_matrix (seed:W8.t Array32.t, transposed:W64.t) : W16.t Array768.t *
-                                                              W16.t Array768.t *
-                                                              W16.t Array768.t = {
+  proc gen_matrix (seed:W8.t Array32.t, transposed:W64.t) : W16.t Array768.t *
+                                                            W16.t Array768.t *
+                                                            W16.t Array768.t = {
     var aux: int;
     
     var r0:W16.t Array768.t;
@@ -1351,14 +1446,14 @@ module M = {
         extseed.[32] <- (W8.of_int 0);
         extseed.[(32 + 1)] <- (W8.of_int j);
       }
-      state <@ _shake128_absorb34 (state, extseed);
+      state <@ shake128_absorb34 (state, extseed);
       ctr <- (W64.of_int 0);
       
       while ((ctr \ult (W64.of_int 256))) {
         sctr <- ctr;
-        (state, buf) <@ _shake128_squeezeblock (state, buf);
+        (state, buf) <@ shake128_squeezeblock (state, buf);
         ctr <- sctr;
-        (ctr, poly) <@ __rej_uniform (poly, ctr, buf);
+        (ctr, poly) <@ rej_uniform (poly, ctr, buf);
       }
       k <- (W64.of_int 0);
       l <- (W64.of_int (j * 256));
@@ -1381,14 +1476,14 @@ module M = {
         extseed.[32] <- (W8.of_int 1);
         extseed.[(32 + 1)] <- (W8.of_int j);
       }
-      state <@ _shake128_absorb34 (state, extseed);
+      state <@ shake128_absorb34 (state, extseed);
       ctr <- (W64.of_int 0);
       
       while ((ctr \ult (W64.of_int 256))) {
         sctr <- ctr;
-        (state, buf) <@ _shake128_squeezeblock (state, buf);
+        (state, buf) <@ shake128_squeezeblock (state, buf);
         ctr <- sctr;
-        (ctr, poly) <@ __rej_uniform (poly, ctr, buf);
+        (ctr, poly) <@ rej_uniform (poly, ctr, buf);
       }
       k <- (W64.of_int 0);
       l <- (W64.of_int (j * 256));
@@ -1411,14 +1506,14 @@ module M = {
         extseed.[32] <- (W8.of_int 2);
         extseed.[(32 + 1)] <- (W8.of_int j);
       }
-      state <@ _shake128_absorb34 (state, extseed);
+      state <@ shake128_absorb34 (state, extseed);
       ctr <- (W64.of_int 0);
       
       while ((ctr \ult (W64.of_int 256))) {
         sctr <- ctr;
-        (state, buf) <@ _shake128_squeezeblock (state, buf);
+        (state, buf) <@ shake128_squeezeblock (state, buf);
         ctr <- sctr;
-        (ctr, poly) <@ __rej_uniform (poly, ctr, buf);
+        (ctr, poly) <@ rej_uniform (poly, ctr, buf);
       }
       k <- (W64.of_int 0);
       l <- (W64.of_int (j * 256));
@@ -1432,6 +1527,105 @@ module M = {
       j <- j + 1;
     }
     return (r0, r1, r2);
+  }
+  
+  proc indcpa_keypair_jazz (pkp:W64.t, skp:W64.t, randomnessp:W64.t) : unit = {
+    
+    var spkp:W64.t;
+    var sskp:W64.t;
+    var i:W64.t;
+    var c:W8.t;
+    var inbuf:W8.t Array32.t;
+    var buf:W8.t Array64.t;
+    var j:W64.t;
+    var publicseed:W8.t Array32.t;
+    var noiseseed:W8.t Array32.t;
+    var zero:W64.t;
+    var a0:W16.t Array768.t;
+    var a1:W16.t Array768.t;
+    var a2:W16.t Array768.t;
+    var nonce:W8.t;
+    var poly0:W16.t Array256.t;
+    var poly1:W16.t Array256.t;
+    var poly2:W16.t Array256.t;
+    var skpv:W16.t Array768.t;
+    var e:W16.t Array768.t;
+    var pkpv:W16.t Array768.t;
+    a0 <- witness;
+    a1 <- witness;
+    a2 <- witness;
+    buf <- witness;
+    e <- witness;
+    inbuf <- witness;
+    noiseseed <- witness;
+    pkpv <- witness;
+    poly0 <- witness;
+    poly1 <- witness;
+    poly2 <- witness;
+    publicseed <- witness;
+    skpv <- witness;
+    spkp <- pkp;
+    sskp <- skp;
+    i <- (W64.of_int 0);
+    
+    while ((i \ult (W64.of_int 32))) {
+      c <- (loadW8 Glob.mem (W64.to_uint (randomnessp + i)));
+      inbuf.[(W64.to_uint i)] <- c;
+      i <- (i + (W64.of_int 1));
+    }
+    buf <@ sha3512_32 (buf, inbuf);
+    i <- (W64.of_int 0);
+    j <- (W64.of_int 32);
+    
+    while ((i \ult (W64.of_int 32))) {
+      c <- buf.[(W64.to_uint i)];
+      publicseed.[(W64.to_uint i)] <- c;
+      c <- buf.[(W64.to_uint j)];
+      noiseseed.[(W64.to_uint i)] <- c;
+      i <- (i + (W64.of_int 1));
+      j <- (j + (W64.of_int 1));
+    }
+    zero <- (W64.of_int 0);
+    (a0, a1, a2) <@ gen_matrix (publicseed, zero);
+    nonce <- (W8.of_int 0);
+    poly0 <@ poly_getnoise (poly0, noiseseed, nonce);
+    nonce <- (W8.of_int 1);
+    poly1 <@ poly_getnoise (poly1, noiseseed, nonce);
+    nonce <- (W8.of_int 2);
+    poly2 <@ poly_getnoise (poly2, noiseseed, nonce);
+    skpv <@ polyvec_frompolys (poly0, poly1, poly2);
+    nonce <- (W8.of_int 3);
+    poly0 <@ poly_getnoise (poly0, noiseseed, nonce);
+    nonce <- (W8.of_int 4);
+    poly1 <@ poly_getnoise (poly1, noiseseed, nonce);
+    nonce <- (W8.of_int 5);
+    poly2 <@ poly_getnoise (poly2, noiseseed, nonce);
+    e <@ polyvec_frompolys (poly0, poly1, poly2);
+    skpv <@ polyvec_ntt (skpv);
+    e <@ polyvec_ntt (e);
+    poly0 <@ polyvec_pointwise_acc (a0, skpv);
+    poly0 <@ poly_frommont (poly0);
+    poly1 <@ polyvec_pointwise_acc (a1, skpv);
+    poly1 <@ poly_frommont (poly1);
+    poly2 <@ polyvec_pointwise_acc (a2, skpv);
+    poly2 <@ poly_frommont (poly2);
+    pkpv <@ polyvec_frompolys (poly0, poly1, poly2);
+    pkpv <@ polyvec_add2 (pkpv, e);
+    pkpv <@ polyvec_reduce (pkpv);
+    pkp <- spkp;
+    skp <- sskp;
+    polyvec_tobytes (skp, skpv);
+    polyvec_tobytes (pkp, pkpv);
+    i <- (W64.of_int 0);
+    pkp <- (pkp + (W64.of_int (3 * 384)));
+    
+    while ((i \ult (W64.of_int 32))) {
+      c <- publicseed.[(W64.to_uint i)];
+      Glob.mem <- storeW8 Glob.mem (W64.to_uint (pkp + (W64.of_int 0))) c;
+      pkp <- (pkp + (W64.of_int 1));
+      i <- (i + (W64.of_int 1));
+    }
+    return ();
   }
   
   proc indcpa_enc_jazz (ctp:W64.t, msgp:W64.t, pkp:W64.t, coinsp:W64.t) : unit = {
@@ -1479,7 +1673,7 @@ module M = {
       noiseseed.[(W64.to_uint i)] <- c;
       i <- (i + (W64.of_int 1));
     }
-    pkpv <@ __polyvec_frombytes (pkp);
+    pkpv <@ polyvec_frombytes (pkp);
     i <- (W64.of_int 0);
     pkp <- (pkp + (W64.of_int (3 * 384)));
     
@@ -1489,42 +1683,42 @@ module M = {
       pkp <- (pkp + (W64.of_int 1));
       i <- (i + (W64.of_int 1));
     }
-    k <@ _poly_frommsg (k, msgp);
+    k <@ poly_frommsg (k, msgp);
     one <- (W64.of_int 1);
-    (at0, at1, at2) <@ __gen_matrix (publicseed, one);
+    (at0, at1, at2) <@ gen_matrix (publicseed, one);
     nonce <- (W8.of_int 0);
-    poly0 <@ _poly_getnoise (poly0, noiseseed, nonce);
+    poly0 <@ poly_getnoise (poly0, noiseseed, nonce);
     nonce <- (W8.of_int 1);
-    poly1 <@ _poly_getnoise (poly1, noiseseed, nonce);
+    poly1 <@ poly_getnoise (poly1, noiseseed, nonce);
     nonce <- (W8.of_int 2);
-    poly2 <@ _poly_getnoise (poly2, noiseseed, nonce);
-    sp_0 <@ __polyvec_frompolys (poly0, poly1, poly2);
+    poly2 <@ poly_getnoise (poly2, noiseseed, nonce);
+    sp_0 <@ polyvec_frompolys (poly0, poly1, poly2);
     nonce <- (W8.of_int 3);
-    poly0 <@ _poly_getnoise (poly0, noiseseed, nonce);
+    poly0 <@ poly_getnoise (poly0, noiseseed, nonce);
     nonce <- (W8.of_int 4);
-    poly1 <@ _poly_getnoise (poly1, noiseseed, nonce);
+    poly1 <@ poly_getnoise (poly1, noiseseed, nonce);
     nonce <- (W8.of_int 5);
-    poly2 <@ _poly_getnoise (poly2, noiseseed, nonce);
-    ep <@ __polyvec_frompolys (poly0, poly1, poly2);
+    poly2 <@ poly_getnoise (poly2, noiseseed, nonce);
+    ep <@ polyvec_frompolys (poly0, poly1, poly2);
     nonce <- (W8.of_int 6);
-    epp <@ _poly_getnoise (epp, noiseseed, nonce);
-    sp_0 <@ __polyvec_ntt (sp_0);
-    poly0 <@ __polyvec_pointwise_acc (at0, sp_0);
-    poly1 <@ __polyvec_pointwise_acc (at1, sp_0);
-    poly2 <@ __polyvec_pointwise_acc (at2, sp_0);
-    bp <@ __polyvec_frompolys (poly0, poly1, poly2);
-    v <@ __polyvec_pointwise_acc (pkpv, sp_0);
-    bp <@ __polyvec_invntt (bp);
-    v <@ _poly_invntt (v);
-    bp <@ __polyvec_add2 (bp, ep);
-    v <@ _poly_add2 (v, epp);
-    v <@ _poly_add2 (v, k);
-    bp <@ __polyvec_reduce (bp);
-    v <@ __poly_reduce (v);
+    epp <@ poly_getnoise (epp, noiseseed, nonce);
+    sp_0 <@ polyvec_ntt (sp_0);
+    poly0 <@ polyvec_pointwise_acc (at0, sp_0);
+    poly1 <@ polyvec_pointwise_acc (at1, sp_0);
+    poly2 <@ polyvec_pointwise_acc (at2, sp_0);
+    bp <@ polyvec_frompolys (poly0, poly1, poly2);
+    v <@ polyvec_pointwise_acc (pkpv, sp_0);
+    bp <@ polyvec_invntt (bp);
+    v <@ poly_invntt (v);
+    bp <@ polyvec_add2 (bp, ep);
+    v <@ poly_add2 (v, epp);
+    v <@ poly_add2 (v, k);
+    bp <@ polyvec_reduce (bp);
+    v <@ poly_reduce (v);
     ctp <- sctp;
-    __polyvec_compress (ctp, bp);
+    polyvec_compress (ctp, bp);
     ctp <- (ctp + (W64.of_int (3 * 320)));
-    v <@ _poly_compress (ctp, v);
+    v <@ poly_compress (ctp, v);
     return ();
   }
   
@@ -1540,16 +1734,16 @@ module M = {
     skpv <- witness;
     t <- witness;
     v <- witness;
-    bp <@ __polyvec_decompress (ctp);
+    bp <@ polyvec_decompress (ctp);
     ctp <- (ctp + (W64.of_int (3 * 320)));
-    v <@ _poly_decompress (v, ctp);
-    skpv <@ __polyvec_frombytes (skp);
-    bp <@ __polyvec_ntt (bp);
-    t <@ __polyvec_pointwise_acc (skpv, bp);
-    t <@ _poly_invntt (t);
-    mp <@ _poly_sub (mp, v, t);
-    mp <@ __poly_reduce (mp);
-    mp <@ _poly_tomsg (msgp, mp);
+    v <@ poly_decompress (v, ctp);
+    skpv <@ polyvec_frombytes (skp);
+    bp <@ polyvec_ntt (bp);
+    t <@ polyvec_pointwise_acc (skpv, bp);
+    t <@ poly_invntt (t);
+    mp <@ poly_sub (mp, v, t);
+    mp <@ poly_reduce (mp);
+    mp <@ poly_tomsg (msgp, mp);
     return ();
   }
 }.
