proof/correctness/Fq.ec
@@ -249,7 +249,7 @@ smt().
 qed.
 
 lemma fqmul_corr_h _a _b: 
-   hoare[ Jindcpa.M.__fqmul : to_sint a = _a /\ to_sint b = _b ==> 
+   hoare[ Jindcpa.M.fqmul : to_sint a = _a /\ to_sint b = _b ==> 
    to_sint res = SREDC (_a * _b)].
 proof.
 proc.
@@ -269,10 +269,10 @@ by rewrite W32.of_sintK /=; smt(qE).
 qed.
 
 lemma fqmul_ll :
-  islossless M.__fqmul by proc; islossless.
+  islossless M.fqmul by proc; islossless.
 
 lemma fqmul_corr _a _b :
-  phoare [ M.__fqmul : 
+  phoare [ M.fqmul : 
      W16.to_sint a = _a /\ W16.to_sint b = _b ==> 
          W16.to_sint res = SREDC (_a * _b)] = 1%r.
 proof. by conseq fqmul_ll (fqmul_corr_h _a _b). qed.
@@ -394,7 +394,7 @@ qed.
 
 
 lemma barrett_reduce_corr_h _a :
-  hoare [ M.__barrett_reduce : 
+  hoare [ M.barrett_reduce : 
      W16.to_sint a = _a  ==> 
          W16.to_sint res = BREDC _a 26].
 proof.
@@ -442,10 +442,10 @@ by smt(@W16 qE).
 qed.
 
 lemma barrett_reduce_ll :
-  islossless M.__barrett_reduce by proc; islossless.
+  islossless M.barrett_reduce by proc; islossless.
 
 lemma barrett_reduce_corr _a :
-  phoare [ M.__barrett_reduce : 
+  phoare [ M.barrett_reduce : 
      W16.to_sint a = _a  ==> 
          W16.to_sint res = BREDC _a 26] = 1%r.
 proof. by conseq barrett_reduce_ll (barrett_reduce_corr_h _a). qed.
